generalize reorder tapes
allow specifying list of "default" tapes. the reasoning on steps now holds for arbitrary base tape contents, and not only empty tapes. this allows potential use for composition without requiring the first TM to clean up its tapes, which in general I consider not feasible

papers/116_stefan_rass/TM.thy
@@ -405,6 +405,7 @@ definition tape_write :: "'s tp_symbol \<Rightarrow> 's tape \<Rightarrow> 's ta
   where "tape_write s tp = \<langle>left tp|s|right tp\<rangle>"
 
 corollary tape_write_simps[simp]: "tape_write s \<langle>l|h|r\<rangle> = \<langle>l|s|r\<rangle>" unfolding tape_write_def by simp
+corollary tape_write_id[simp]: "tape_write (head tp) tp = tp" by (induction tp) simp
 
 
 text\<open>Write a symbol, then move the head.\<close>
@@ -414,6 +415,9 @@ definition tape_action :: "('s tp_symbol \<times> head_move) \<Rightarrow> 's ta
 
 corollary tape_action_altdef: "tape_action (s, m) = tape_shift m \<circ> tape_write s"
   unfolding tape_action_def by auto
+
+lemma tape_action_id[simp]: "tape_action (head tp, No_Shift) tp = tp"
+  unfolding tape_action_altdef by simp
 
 end \<comment> \<open>\<^locale>\<open>TM_abbrevs\<close>\<close>
 
@@ -507,158 +511,148 @@ end \<comment> \<open>\<^locale>\<open>TM\<close>\<close>
 
 subsubsection\<open>Reordering Tapes\<close>
 
-definition reorder :: "nat option list \<Rightarrow> 'a \<Rightarrow> 'a list \<Rightarrow> 'a list"
-  where "reorder is x xs = map (\<lambda>i'. case i' of None \<Rightarrow> x | Some i \<Rightarrow> nth_or i x xs) is"
 
-value "reorder [Some 0, Some 2, Some 1, None] x [a,b,c]"
+definition reorder :: "(nat \<Rightarrow> nat option) \<Rightarrow> 'a list \<Rightarrow> 'a list \<Rightarrow> 'a list"
+  where "reorder p xs ys = map2 (\<lambda>i x. case p i of None \<Rightarrow> x | Some i' \<Rightarrow> nth_or i' x ys) [0..<length xs] xs"
 
+value "reorder (\<lambda>i. [Some 0, Some 2, Some 1, None]!i) (x\<up>4) [a,b,c]"
 
-lemma reorder_length[simp]: "length (reorder is x xs) = length is" unfolding reorder_def by simp
+lemma reorder_length[simp]: "length (reorder p xs ys) = length xs" unfolding reorder_def by simp
 
-lemma reorder_map[simp]: "map f (reorder is x xs) = reorder is (f x) (map f xs)"
-  unfolding reorder_def map_map comp_def option.case_distrib nth_or_map ..
+lemma reorder_Nil[simp]: "reorder p xs [] = xs"
+  unfolding reorder_def nth_or_Nil case_option_same prod.snd_def[symmetric] by simp
 
-lemma reorder_nth:
-  assumes "i < length is"
-  shows "reorder is x xs ! i = (case is ! i of None \<Rightarrow> x | Some i \<Rightarrow> nth_or i x xs)"
-  unfolding reorder_def nth_map[OF assms] ..
+lemma reorder_nth[simp]:
+  assumes "i < length xs"
+  shows "reorder p xs ys ! i = (case p i of None \<Rightarrow> xs ! i | Some i' \<Rightarrow> nth_or i' (xs ! i) ys)"
+  using assms unfolding reorder_def by (subst nth_map2) auto
 
-lemma reorder_zip:
-  assumes [simp]: "length xs = length ys"
-  shows "reorder is (x, y) (zip xs ys) = zip (reorder is x xs) (reorder is y ys)"
-  unfolding reorder_def zip_map_map map2_same
-proof (intro list.map_cong0)
-  fix i'
-  show "(case i' of None \<Rightarrow> (x, y) | Some i \<Rightarrow> nth_or i (x, y) (zip xs ys)) =
-    (case i' of None \<Rightarrow> x | Some i \<Rightarrow> nth_or i x xs, case i' of None \<Rightarrow> y | Some i \<Rightarrow> nth_or i y ys)"
-  proof (induction i', unfold option.case)
-    fix i
-    show "nth_or i (x, y) (zip xs ys) = (nth_or i x xs, nth_or i y ys)"
-      by (cases "i < length ys") auto
-  qed simp
+lemma reorder_map[simp]: "map f (reorder p xs ys) = reorder p (map f xs) (map f ys)"
+proof -
+  have "map f (reorder p xs ys) = map (\<lambda>(i, x). f (case p i of None \<Rightarrow> x | Some i' \<Rightarrow> nth_or i' x ys)) (zip [0..<length xs] xs)"
+    unfolding reorder_def map_map comp_def by force
+  also have "... = map2 (\<lambda>i x. case p i of None \<Rightarrow> f x | Some i' \<Rightarrow> nth_or i' (f x) (map f ys)) [0..<length xs] xs"
+    unfolding option.case_distrib nth_or_map ..
+  also have "... = map ((\<lambda>(i, x). case p i of None \<Rightarrow> x | Some i' \<Rightarrow> nth_or i' x (map f ys)) \<circ> (\<lambda>(i, x). (i, f x))) (zip [0..<length xs] xs)"
+    by fastforce
+  also have "... = map (\<lambda>(i, x). case p i of None \<Rightarrow> x | Some i' \<Rightarrow> nth_or i' x (map f ys)) (map (\<lambda>(i, x). (i, f x)) (zip [0..<length xs] xs))"
+    by force
+  also have "... = map2 (\<lambda>i x. case p i of None \<Rightarrow> x | Some i' \<Rightarrow> nth_or i' x (map f ys)) [0..<length xs] (map f xs)"
+    unfolding zip_map_map[symmetric] list.map_ident ..
+  also have "... = reorder p (map f xs) (map f ys)" unfolding reorder_def by simp
+  finally show ?thesis .
 qed
 
-lemma reorder_map2:
-  assumes ls: "length xs = length ys"
-    and fxy: "fxy = f x y"
-  shows "reorder is fxy (map2 f xs ys) = map2 f (reorder is x xs) (reorder is y ys)"
-  unfolding fxy reorder_zip[OF ls, symmetric] reorder_map prod.case ..
+
+(* TODO are both xs and ys needed here? in practice they seem always be identical *)
+definition reorder_inv :: "(nat \<Rightarrow> nat option) \<Rightarrow> 'a list \<Rightarrow> 'a list"
+  where "reorder_inv p ys = map
+    (\<lambda>i. ys ! (LEAST i'. i'<length ys \<and> p i' = Some i))
+    [0..<Suc (Max (Option.these (p ` {0..<length ys})))]"
 
 
-definition reorder_inv :: "nat option list \<Rightarrow> 'a \<Rightarrow> 'a list \<Rightarrow> 'a list"
-  where "reorder_inv is x xs = map
-    (\<lambda>i. case find (\<lambda>(i', x). x = Some i) (List.enumerate 0 is)
-         of None \<Rightarrow> x
-          | Some i' \<Rightarrow> nth_or (fst i') x xs )
-    [0..<if set is \<subseteq> {None} then 0 else Suc (Max (Option.these (set is)))]"
-
-value "reorder_inv [Some 0, Some 2, Some 1, None] x [a, c, b, x]"
-
+lemma card_these_helper: "card (Option.these (f ` {0..<n})) \<le> n"
+proof -
+  have "card (Option.these (f ` {0..<n})) \<le> card (f ` {0..<n})" by (rule card_these) blast
+  also have "... \<le> card {0..<n}" by (rule card_image_le) blast
+  also have "... \<le> n" by simp
+  finally show ?thesis .
+qed
 
 lemma reorder_inv:
-  assumes items_match: "Option.these (set is) = {0..<length xs}"
-  shows "reorder_inv is x (reorder is x xs) = xs"
+  assumes "ys \<noteq> []"
+    and items_match: "Option.these (p ` {0..<length xs}) = {0..<length ys}"
+  shows "reorder_inv p (reorder p xs ys) = ys"
 proof -
-  have *: "(if set is \<subseteq> {None} then 0 else Suc (Max (Option.these (set is)))) = length xs"
-  proof (rule ifI)
-    assume "set is \<subseteq> {None}"
-    then have *: "Option.these (set is) = {}" unfolding Option.these_def by blast
-    from items_match show "0 = length xs" unfolding * by simp
-  next
-    assume "\<not> set is \<subseteq> {None}"
-    then have "Option.these (set is) \<noteq> {}" unfolding subset_singleton_iff these_empty_eq .
-    then have "length xs > 0" unfolding items_match atLeastLessThan_upt by force
-    then show "Suc (Max (Option.these (set is))) = length xs"
-      unfolding items_match Max_atLeastLessThan_nat[OF \<open>length xs > 0\<close>] by auto
+  from \<open>ys \<noteq> []\<close> have "length ys > 0" by simp
+
+  define zs where "zs \<equiv> reorder p xs ys"
+  have lz: "length zs = length xs" unfolding zs_def reorder_length ..
+
+  from \<open>length ys > 0\<close>have *:
+    "Suc (Max (Option.these (p ` {0..<length xs}))) = length ys"
+    unfolding items_match Max_atLeastLessThan_nat[OF \<open>length ys > 0\<close>] by auto
+
+  have "length ys = card (Option.these (p ` {0..<length xs}))" unfolding items_match by simp
+  also have "... \<le> length xs" by (rule card_these_helper)
+  finally have ls: "length xs \<ge> length ys" .
+  then have mls: "min (length [0..<length ys]) (length xs) = length ys" by simp
+
+  have "reorder_inv p (reorder p xs ys) = map ((!) ys) [0..<length ys]"
+    unfolding reorder_inv_def zs_def[symmetric] lz *
+  proof (intro list.map_cong0)
+    fix n assume "n \<in> set [0..<length ys]"
+    then have [simp]: "n < length ys" by simp
+    then have *: "[0..<length ys] ! n = n" by simp
+
+    define i where "i = (LEAST i. i < length xs \<and> p i = Some n)"
+
+    from \<open>n < length ys\<close> have "n \<in> Option.these (p ` {0..<length xs})" unfolding items_match by simp
+    then have "Some n \<in> p ` {0..<length xs}" unfolding these_altdef by force
+    then have [simp]: "\<exists>i. i < length xs \<and> p i = Some n" unfolding image_iff by fastforce
+
+    then have "i < length xs \<and> p i = Some n" unfolding i_def by (rule LeastI_ex)
+    then have [simp]: "i < length xs" and [simp]: "p i = Some n" by blast+
+    then have [simp]: "[0..<length xs] ! i = i" by simp
+
+    have **: "nth_or i x (map2 (\<lambda>x y. case p x of None \<Rightarrow> y | Some i' \<Rightarrow> nth_or i' y ys) [0..<length xs] xs)
+        = ys ! n" for x by simp
+
+    show "zs ! (LEAST i'. i' < length xs \<and> p i' = Some n) = ys ! n"
+      unfolding i_def[symmetric] zs_def reorder_def by simp
   qed
-
-  show ?thesis unfolding reorder_def unfolding reorder_inv_def *
-  proof (intro map_nthI)
-    fix n assume "n < length xs"
-
-    define i where "i = (LEAST i. i < length is \<and> is ! i = Some n)"
-
-    from \<open>n < length xs\<close> have "n \<in> Option.these (set is)" unfolding items_match by simp
-    then have "Some n \<in> set is" unfolding Option.these_def by force
-    then have "\<exists>i<length is. is ! i = Some n" unfolding in_set_conv_nth .
-
-    then have "i < length is \<and> is ! i = Some n" unfolding i_def by (rule LeastI_ex)
-    then have "i < length is" and "is ! i = Some n" by blast+
-
-    have *: "find (\<lambda>(i', x). x = Some n) (List.enumerate 0 is) = Some (i, Some n)"
-      unfolding find_Some_iff
-    proof (intro exI conjI allI impI)
-      from \<open>i < length is\<close> show "i < length (List.enumerate 0 is)" by simp
-      show *[symmetric]: "(i, Some n) = List.enumerate 0 is ! i"
-        unfolding nth_enumerate_eq[OF \<open>i < length is\<close>] \<open>is ! i = Some n\<close> by simp
-      show "case List.enumerate 0 is ! i of (i', x) \<Rightarrow> x = Some n" unfolding * by blast
-      fix j assume "j < i"
-      with \<open>i < length is\<close> have "j < length is" by simp
-
-      from \<open>j < i\<close> have "\<not> (j < length is \<and> is ! j = Some n)" unfolding i_def by (rule not_less_Least)
-      with \<open>j < length is\<close> have "is ! j \<noteq> Some n" by blast
-
-      then show "\<not> (case List.enumerate 0 is ! j of (i', x) \<Rightarrow> x = Some n)"
-        unfolding nth_enumerate_eq[OF \<open>j < length is\<close>] by blast
-    qed
-
-    have "(case find (\<lambda>(i', x). x = Some n) (List.enumerate 0 is) of None \<Rightarrow> x
-          | Some i' \<Rightarrow> nth_or (fst i') x (map (case_option x (\<lambda>i. nth_or i x xs)) is)) =
-         nth_or i x (map (case_option x (\<lambda>i. nth_or i x xs)) is)"
-      unfolding * option.case(2) fst_conv ..
-    also have "... = map (case_option x (\<lambda>i. nth_or i x xs)) is ! i"
-      using \<open>i < length is\<close> by (subst nth_or_val) auto
-    also have "... = nth_or n x xs"
-      unfolding nth_map[OF \<open>i < length is\<close>] \<open>is ! i = Some n\<close> option.case(2) ..
-    also have "... = xs ! n" using \<open>n < length xs\<close> by (rule nth_or_val)
-    finally show "(case find (\<lambda>(i', x). x = Some n) (List.enumerate 0 is) of None \<Rightarrow> x
-      | Some i' \<Rightarrow> nth_or (fst i') x (map (case_option x (\<lambda>i. nth_or i x xs)) is)) = xs ! n" .
-  qed
+  then show ?thesis unfolding map_nth .
 qed
 
 (* definition reorder_fun *)
   (* where "reorder_fun f k l = map (\<lambda>i. if i \<in> f ` {0..<l} then Some (inv_into {0..<l} f i) else None) [0..<k]" *)
 
+definition reorder_config :: "(nat \<Rightarrow> nat option) \<Rightarrow> 's tape list \<Rightarrow> ('q, 's) TM_config \<Rightarrow> ('q, 's) TM_config"
+  where "reorder_config p tps c = \<lparr> state = state c, tapes = reorder p tps (tapes c) \<rparr>"
 
-
-
-definition reorder_config :: "(nat option list) \<Rightarrow> ('q, 's) TM_config \<Rightarrow> ('q, 's) TM_config"
-  where "reorder_config is c = \<lparr> state = state c, tapes = reorder is empty_tape (tapes c) \<rparr>"
-
-lemma reorder_config_length[simp]: "length (tapes (reorder_config is c)) = length is"
+lemma reorder_config_length[simp]: "length (tapes (reorder_config p tps c)) = length tps"
   unfolding reorder_config_def TM_config.simps reorder_length ..
 
 lemma reorder_config_simps[simp]:
-  shows reorder_config_state: "state (reorder_config is c) = state c"
-    and reorder_config_tapes: "tapes (reorder_config is c) = reorder is empty_tape (tapes c)"
+  shows reorder_config_state: "state (reorder_config p tps c) = state c"
+    and reorder_config_tapes: "tapes (reorder_config p tps c) = reorder p tps (tapes c)"
   unfolding reorder_config_def by simp_all
-
 
 
 locale reorder_tapes =
   fixes M :: "('q, 's::finite) TM"
-    and "is" :: "nat option list"
-  assumes min_len: "length is \<ge> TM.tape_count M"
-    and items_match: "Option.these (set is) = {0..<TM.tape_count M}"
+    and p :: "nat \<Rightarrow> nat option"
+    and k' :: nat
+  assumes items_match: "Option.these (p ` {0..<k'}) = {0..<TM.tape_count M}"
 begin
 sublocale TM .
 
+lemma k_k': "k \<le> k'"
+proof -
+  have "k = card {0..<k}" by simp
+  also have "... = card (Option.these (p ` {0..<k'}))" unfolding items_match ..
+  also have "... \<le> card (p ` {0..<k'})" by (rule card_these) blast
+  also have "... \<le> card {0..<k'}" by (rule card_image_le) blast
+  also have "... = k'" by simp
+  finally show "k \<le> k'" .
+qed
+
 definition reorder_tapes_rec :: "('q, 's) TM_record"
   where "reorder_tapes_rec \<equiv>
-    let h = reorder_inv is Bk in
+    let h = reorder_inv p in
     M_rec \<lparr>
-      tape_count := length is,
+      tape_count := k',
       next_state := \<lambda>q hds. \<delta>\<^sub>q q (h hds),
-      next_write := \<lambda>q hds i. case nth_or i None is of Some i \<Rightarrow> (\<delta>\<^sub>w q (h hds) i) | None \<Rightarrow> hds ! i,
-      next_move  := \<lambda>q hds i. case nth_or i None is of Some i \<Rightarrow> (\<delta>\<^sub>m q (h hds) i) | None \<Rightarrow> No_Shift
+      next_write := \<lambda>q hds i. case p i of Some i \<Rightarrow> (\<delta>\<^sub>w q (h hds) i) | None \<Rightarrow> hds ! i,
+      next_move  := \<lambda>q hds i. case p i of Some i \<Rightarrow> (\<delta>\<^sub>m q (h hds) i) | None \<Rightarrow> No_Shift
     \<rparr>"
 
 lemma reorder_tapes_rec_simps: "reorder_tapes_rec = \<lparr>
-  TM_record.tape_count = length is,
+  TM_record.tape_count = k',
   states = Q, initial_state = q\<^sub>0, final_states = F, accepting_states = F\<^sup>+,
-  next_state = \<lambda>q hds. \<delta>\<^sub>q q (reorder_inv is Bk hds),
-  next_write = \<lambda>q hds i. case nth_or i None is of Some i \<Rightarrow> (\<delta>\<^sub>w q (reorder_inv is Bk hds) i) | None \<Rightarrow> hds ! i,
-  next_move  = \<lambda>q hds i. case nth_or i None is of Some i \<Rightarrow> (\<delta>\<^sub>m q (reorder_inv is Bk hds) i) | None \<Rightarrow> No_Shift
+  next_state = \<lambda>q hds. \<delta>\<^sub>q q (reorder_inv p hds),
+  next_write = \<lambda>q hds i. case p i of Some i \<Rightarrow> (\<delta>\<^sub>w q (reorder_inv p hds) i) | None \<Rightarrow> hds ! i,
+  next_move  = \<lambda>q hds i. case p i of Some i \<Rightarrow> (\<delta>\<^sub>m q (reorder_inv p hds) i) | None \<Rightarrow> No_Shift
 \<rparr>" unfolding reorder_tapes_rec_def Let_def by simp
 
 definition [simp]: "M' \<equiv> Abs_TM reorder_tapes_rec"
@@ -666,10 +660,8 @@ definition [simp]: "M' \<equiv> Abs_TM reorder_tapes_rec"
 lemma M'_valid: "is_valid_TM reorder_tapes_rec"
   unfolding reorder_tapes_rec_simps
 proof (unfold_locales, unfold TM_record.simps)
-  from min_len at_least_one_tape show "length is \<ge> 1" by simp
+  from at_least_one_tape and k_k' show "1 \<le> k'" by simp
 qed (fact state_axioms)+
-
-(* corollary M'_valid2[intro, simp]: "reorder_tapes_rec \<in> {M. is_valid_TM M}" using M'_valid .. *)
 
 sublocale M': TM M' .
 
@@ -677,13 +669,12 @@ lemma M'_rec: "M'.M_rec = reorder_tapes_rec" using Abs_TM_inverse M'_valid by au
 lemmas M'_simps = M'.TM_fields_defs M'_rec reorder_tapes_rec_simps TM_record.simps
 
 lemma M'_F: "M'.F = F" unfolding M'_simps ..
-lemma M'_k: "M'.k = length is" unfolding M'_simps ..
-
-lemma r_len: "length (reorder is x xs) = M'.k" unfolding M'_k by (fact reorder_length)
+lemma M'_k: "M'.k = k'" unfolding M'_simps ..
 
 lemma reorder_steps:
   assumes "wf_config c"
-  shows "M'.step (reorder_config is c) = reorder_config is (step c)"
+    and "M'.wf_config c'"
+  shows "M'.step (reorder_config p (tapes c') c) = reorder_config p (tapes c') (step c)"
     (is "M'.step (?rc c) = ?rc (step c)")
 proof (cases "is_final c")
   assume "is_final c"
@@ -696,14 +687,19 @@ next
   let ?q = "state c" and ?q' = "state ?c'"
   let ?tps = "tapes c" and ?hds = "heads c"
 
-  let ?r = "reorder is"
-  let ?hds' = "?r Bk ?hds" and ?tps' = "?r \<langle>\<rangle> ?tps"
+  let ?r = "reorder p"
+  let ?hds' = "?r (heads c') ?hds" and ?tps' = "?r (tapes c') ?tps"
 
   from \<open>wf_config c\<close> have l_tps: "length (tapes c) = k" by simp
   then have l_hds: "length (heads c) = k" by simp
-  have "Option.these (set is) = {0..<length (heads c)}"
-    unfolding \<open>length (heads c) = k\<close> by (fact items_match)
-  note r_inv_hds[simp] = reorder_inv[OF this]
+  from \<open>M'.wf_config c'\<close> have l_tps': "length (tapes c') = k'" unfolding TM.wf_config_def M'_k .
+  then have l_hds': "length (heads c') = k'" by simp
+
+  (* have l_hds'': "length ?hds' = k'" unfolding reorder_length l_hds' M'_k .. *)
+  from at_least_one_tape have "?hds \<noteq> []" unfolding length_0_conv[symmetric] l_hds by simp
+  moreover have "Option.these (p ` {0..<length (heads c')}) = {0..<length ?hds}"
+    unfolding l_hds l_hds' unfolding items_match ..
+  ultimately have r_inv_hds[simp]: "reorder_inv p (reorder p (heads c') ?hds) = ?hds" by (rule reorder_inv)
 
   assume "\<not> is_final c"
   then have "\<not> M'.is_final ?c'" unfolding M'_F by simp
@@ -717,43 +713,49 @@ next
       unfolding step_not_final_def Let_def by simp
     finally show "state (M'.step_not_final ?c') = state (?rc (step_not_final c))" .
 
-    have "M'.k \<ge> k" unfolding M'_k by (rule min_len)
-    then have min_k_k': "min k M'.k = k" by simp
-    have l_tps': "length ?tps' = M'.k" unfolding M'_k reorder_config_def TM_config.simps reorder_length ..
+    from k_k' have min_k_k': "min k M'.k = k" unfolding M'_k by simp
+    have lr: "length (reorder p (tapes c') x) = M'.k" for x unfolding reorder_length l_tps' M'_k ..
 
     have "tapes (M'.step_not_final ?c') = map2 tape_action (M'.\<delta>\<^sub>a ?q ?hds') ?tps'"
       unfolding M'.step_not_final_def by (simp add: Let_def)
-    also have "... = ?r \<langle>\<rangle> (map2 tape_action (\<delta>\<^sub>a ?q ?hds) ?tps)"
-    proof (rule TM.step_not_final_eqI)
-      let ?k' = M'.k and ?r = "reorder is"
-      let ?rt = "?r \<langle>\<rangle>" and ?hds'' = "?r None ?hds" let ?tps'' = "?rt ?tps"
-      fix i assume "i < ?k'"
-      then have "i < length is" unfolding M'_k .
-      then have [simp]: "nth_or i x is = is ! i" for x by simp
+    also have "... = ?r (tapes c') (map2 tape_action (\<delta>\<^sub>a ?q ?hds) ?tps)"
+    proof (rule M'.step_not_final_eqI)
+      thm reorder_length
+      let ?r = "reorder p"
+      let ?rt = "?r (tapes c')"
+      fix i assume "i < M'.k"
+      then have [simp]: "i < k'" unfolding M'_k .
+      (* then have [simp]: "nth_or i x is = is ! i" for x by simp *)
 
       show "tape_action (M'.\<delta>\<^sub>w ?q ?hds' i, M'.\<delta>\<^sub>m ?q ?hds' i) (?tps' ! i) =
-        ?r \<langle>\<rangle> (map2 tape_action (\<delta>\<^sub>a ?q ?hds) ?tps) ! i"
-      proof (induction "is ! i")
+        ?rt (map2 tape_action (\<delta>\<^sub>a ?q ?hds) ?tps) ! i"
+      proof (induction "p i")
         case None
-        then have [simp]: "is ! i = None" ..
-        have [simp]: "reorder is x xs ! i = x" for x :: 'x and xs
-          unfolding reorder_nth[OF \<open>i < length is\<close>] by simp
-        then show ?case unfolding M'_simps by (simp add: tape_action_def)
+        then have [simp]: "p i = None" ..
+        from \<open>i < k'\<close> have "reorder p xs ys ! i = xs ! i" if "length xs = k'" for xs ys :: "'x list"
+          using that by simp
+        note * = this[OF l_tps'] this[OF l_hds']
+        from \<open>i < k'\<close> have [simp]: "map head (tapes c') ! i = head (tapes c' ! i)"
+          by (intro nth_map) (unfold l_tps')
+        show ?case unfolding M'_simps * by simp
       next
         case (Some i')
-        then have [simp]: "is ! i = Some i'" ..
+        then have [simp]: "p i = Some i'" ..
 
-        from \<open>i < length is\<close> have "Some i' \<in> set is" unfolding \<open>Some i' = is ! i\<close> by (fact nth_mem)
+
+        from \<open>i < k'\<close> have "i \<in> {0..<k'}" by simp
+        then have "Some i' \<in> p ` {0..<k'}" unfolding \<open>Some i' = p i\<close> by blast
         then have "i' \<in> {0..<k}" unfolding items_match[symmetric] in_these_eq .
         then have [simp]: "i' < k" by simp
 
         then have nth_i': "nth_or i' x xs = xs ! i'" if "length xs = k" for x :: 'x and xs
           unfolding nth_or_def \<open>length xs = k\<close> by (rule if_P)
-        have r_nth_or: "reorder is x xs ! i = nth_or i' x xs" for x :: 'x and xs
-          unfolding reorder_nth[OF \<open>i < length is\<close>] by simp
+        from \<open>i < k'\<close> have "i < length (tapes c')" unfolding l_tps' .
+        have r_nth_or: "reorder p (tapes c') tps ! i = nth_or i' (tapes c' ! i) tps" for tps
+          unfolding reorder_nth[OF \<open>i < length (tapes c')\<close>] by simp
 
-        have \<delta>\<^sub>w': "M'.\<delta>\<^sub>w ?q ?hds'' i = \<delta>\<^sub>w (state c) (heads c) i'"
-         and \<delta>\<^sub>m': "M'.\<delta>\<^sub>m ?q ?hds'' i = \<delta>\<^sub>m (state c) (heads c) i'"
+        have \<delta>\<^sub>w': "M'.\<delta>\<^sub>w ?q ?hds' i = \<delta>\<^sub>w (state c) (heads c) i'"
+         and \<delta>\<^sub>m': "M'.\<delta>\<^sub>m ?q ?hds' i = \<delta>\<^sub>m (state c) (heads c) i'"
           unfolding M'_simps r_inv_hds by simp_all
 
         have "tape_action (M'.\<delta>\<^sub>w ?q ?hds' i, M'.\<delta>\<^sub>m ?q ?hds' i) (?tps' ! i) =
@@ -762,11 +764,11 @@ next
         also have "... = tape_action (\<delta>\<^sub>a ?q ?hds ! i') (?tps ! i')" by simp
         also have "... = map2 tape_action (\<delta>\<^sub>a ?q ?hds) ?tps ! i'"
           by (subst nth_map2) (auto simp add: l_tps)
-        also have "... = ?r \<langle>\<rangle> (map2 tape_action (\<delta>\<^sub>a ?q ?hds) ?tps) ! i"
+        also have "... = ?rt (map2 tape_action (\<delta>\<^sub>a ?q ?hds) ?tps) ! i"
           unfolding r_nth_or by (rule nth_i'[symmetric]) (simp add: l_tps)
         finally show ?case .
       qed
-    qed (fact r_len)+
+    qed (fact lr)+
     also have "... = tapes (?rc (step_not_final c))"
       unfolding M'.step_not_final_def by (simp add: Let_def)
     finally show "tapes (M'.step_not_final ?c') = tapes (?rc (step_not_final c))" .
